src/spl/Assumptions.v
@@ -93,7 +93,7 @@ Section Checker_correct.
   Proof.
     induction c1 as [ |l1 c1 IHc1]; simpl; intros [ |l2 c2]; simpl; auto; try discriminate.
     unfold is_true. rewrite andb_true_iff. intros [H1 H2].
-    rewrite Int63Properties.eqb_spec in H1. now rewrite (IHc1 _ H2), H1.
+    rewrite Int63.eqb_spec in H1. now rewrite (IHc1 _ H2), H1.
   Qed.
 
   Lemma valid_check_clause cid c :
